concurrency/SC_erasure.v
@@ -1,0 +1,1070 @@
+(** ** Erasure from FineConc to a non-angelic SC machine*)
+
+Require Import compcert.lib.Axioms.
+
+Require Import concurrency.sepcomp. Import SepComp.
+Require Import sepcomp.semantics_lemmas.
+
+Require Import concurrency.pos.
+
+From mathcomp.ssreflect Require Import ssreflect ssrbool ssrnat ssrfun eqtype seq fintype finfun.
+Set Implicit Arguments.
+
+(*NOTE: because of redefinition of [val], these imports must appear 
+  after Ssreflect eqtype.*)
+Require Import compcert.common.AST.     (*for typ*)
+Require Import compcert.common.Values. (*for val*)
+Require Import compcert.common.Globalenvs.
+Require Import compcert.common.Events.
+Require Import compcert.common.Memory.
+Require Import compcert.lib.Integers.
+
+Require Import Coq.ZArith.ZArith.
+
+Require Import concurrency.threads_lemmas.
+Require Import concurrency.permissions.
+Require Import concurrency.concurrent_machine.
+Require Import concurrency.memory_lemmas.
+Require Import concurrency.dry_context.
+Require Import concurrency.fineConc_safe.
+Require Import Coqlib.
+Require Import msl.Coqlib2.
+
+Set Bullet Behavior "None".
+Set Bullet Behavior "Strict Subproofs".
+
+(** ** Erasure of Values*)
+Module ValErasure.
+
+  Definition erased_val v1 v2 : Prop :=
+    match v1, v2 with
+    | Vundef, _ => True
+    | v1, v2 => v1 = v2
+    end.
+  
+  Inductive erased_val_list : seq.seq val -> seq.seq val -> Prop :=
+    erased_val_nil : erased_val_list [::] [::]
+  | erased_val_cons : forall (v v' : val) (vl vl' : seq.seq val),
+      erased_val v v' ->
+      erased_val_list vl vl' ->
+      erased_val_list (v :: vl) (v' :: vl').
+
+  Lemma erased_val_refl:
+    forall v, erased_val v v.
+  Proof.
+    destruct v; simpl; auto.
+  Qed.
+
+  Hint Immediate erased_val_refl : erased.
+  Hint Constructors erased_val_list : erased.
+  
+  Lemma erased_val_list_refl:
+    forall vs, erased_val_list vs vs.
+  Proof with eauto with erased.
+    induction vs; simpl...
+  Qed.
+
+  Lemma erased_val_list_decode:
+    forall vals vals' typs,
+      erased_val_list vals vals' ->
+      erased_val_list (decode_longs typs vals) (decode_longs typs vals').
+  Proof.
+    intros.
+    generalize dependent vals.
+    generalize dependent vals'.
+    induction typs; intros; simpl;
+    first by constructor.
+    destruct vals;
+      destruct a; inversion H; subst;
+      try constructor; eauto.
+    destruct vals; inversion H4; subst.
+    constructor.
+    unfold Val.longofwords.
+    destruct v;
+      constructor; eauto;
+      inv H2; try constructor.
+    unfold erased_val in H3.
+    destruct v0; subst; auto;
+    constructor.
+  Qed.
+
+  (** ** Lemmas about erased values*)
+  Lemma erased_val_hiword:
+    forall v v',
+      erased_val v v' ->
+      erased_val (Val.hiword v) (Val.hiword v').
+  Proof.
+    intros;
+    destruct v; simpl; inv H; auto.
+  Qed.
+
+  Lemma erased_val_loword:
+    forall v v',
+      erased_val v v' ->
+      erased_val (Val.loword v) (Val.loword v').
+  Proof.
+    intros;
+    destruct v; simpl; inv H; auto.
+  Qed.
+
+  Lemma erased_val_cmp_bool:
+    forall c v1 v1',
+      v1 <> Vundef ->
+      erased_val v1 v1' ->
+      Val.cmp_bool c v1 Vzero = Val.cmp_bool c v1' Vzero.
+  Proof.
+    intros.
+    destruct v1; try congruence.
+  Qed.
+
+  Hint Resolve erased_val_hiword erased_val_loword : erased.
+
+End ValErasure.
+
+(** ** Memory Erasure*)
+Module MemErasure.
+
+  (** The erased memory is identical for everything but
+       permissions. *)
+  (** NOTE: There is an implicit hypothesis here, which is currently
+  true for the X86 semantics of compcert (and probably for
+  PPC). Undefined values are never stored in the memory. If this was
+  not true we would have to related the contents using [erased_val]*)
+  Local Notation "a # b" := (PMap.get b a) (at level 1).
+
+  Record erasedMem (m m': mem) :=
+    { perm_le:
+        forall b ofs k,
+          Mem.valid_block m' b -> 
+          (Mem.mem_access m')#b ofs k = Some Freeable;
+      erased_contents:
+        (Mem.mem_contents m') = (Mem.mem_contents m);
+      erased_nb: Mem.nextblock m = Mem.nextblock m'
+    }.
+
+  Lemma erasedMem_dilute_1:
+    forall m m',
+      erasedMem m m' ->
+      erasedMem (setMaxPerm m) m'.
+  Proof.
+    intros.
+    inversion H.
+    constructor; auto.
+  Qed.
+
+   Lemma mem_load_erased:
+    forall chunk m m' b ofs pmap v
+      (Hlt: permMapLt pmap (getMaxPerm m))
+      (Hload: Mem.load chunk (restrPermMap Hlt) b ofs = Some v)
+      (Herased: erasedMem m m'),
+      Mem.load chunk m' b ofs = Some v.
+  Proof.
+    intros.
+    inversion Herased.
+    assert (Hreadable := Mem.load_valid_access _ _ _ _ _ Hload).
+    destruct Hreadable.
+    assert (Hreadable': Mem.valid_access m' chunk b ofs Readable).
+    { split; auto.
+      intros ? ?.
+      unfold Mem.perm.
+      rewrite perm_le0.
+      simpl; constructor.
+      eapply MemoryLemmas.load_valid_block in Hload.
+      unfold Mem.valid_block in *. simpl in *.
+      rewrite <- erased_nb0; auto.
+    }
+    Transparent Mem.load.
+    unfold Mem.load in *.
+    destruct (Mem.valid_access_dec m' chunk b ofs Readable);
+      try by exfalso.
+    destruct (Mem.valid_access_dec (restrPermMap Hlt) chunk b ofs Readable);
+      try by discriminate.
+    simpl in *.
+    rewrite erased_contents0; auto.
+    Opaque Mem.load.
+  Qed.
+
+  Lemma mem_store_erased:
+    forall chunk m m' b ofs pmap v m2
+      (Hv: v <> Vundef)
+      (Hlt: permMapLt pmap (getMaxPerm m))
+      (Hstore: Mem.store chunk (restrPermMap Hlt) b ofs v = Some m2)
+      (Herased: erasedMem m m'),
+    exists m2', Mem.store chunk m' b ofs v = Some m2'
+           /\ erasedMem m2 m2'.
+  Proof.
+    intros.
+    destruct Herased.
+    assert (Haccess := Mem.store_valid_access_3 _ _ _ _ _ _ Hstore).
+    assert (Hvalid := Mem.valid_access_valid_block
+                        _ _ _ _ (Mem.valid_access_implies
+                                   _ _ _ _ _ Nonempty Haccess ltac:(constructor))).
+    destruct Haccess.
+    assert (Haccess' : Mem.valid_access m' chunk b ofs Writable).
+    { split; auto.
+      intros ? ?.
+      unfold Mem.perm.
+      rewrite perm_le0.
+      simpl; constructor.
+      unfold Mem.valid_block in *. simpl in *.
+      rewrite <- erased_nb0; auto.
+    }
+    Transparent Mem.store.
+    unfold Mem.store in *.
+    destruct (Mem.valid_access_dec m' chunk b ofs Writable); try by exfalso.
+    destruct (Mem.valid_access_dec (restrPermMap Hlt) chunk b ofs Writable);
+      try by discriminate. simpl in Hstore.
+    inv Hstore.
+    eexists; split; eauto.
+    constructor; simpl; auto.
+    rewrite <- erased_contents0.
+    reflexivity.
+    Opaque Mem.store.
+  Qed.
+
+  Lemma erasedMem_restr:
+    forall m m' pmap (Hlt: permMapLt pmap (getMaxPerm m)),
+      erasedMem m m' ->
+      erasedMem (restrPermMap Hlt) m'.
+  Proof.
+    intros.
+    inversion H.
+    constructor; auto.
+  Qed.
+  
+End MemErasure.
+
+(** Erasure of cores *)
+Module Type CoreErasure (SEM: Semantics).
+  Import SEM ValErasure MemErasure event_semantics.
+  
+  Parameter erasedCores : C -> C -> Prop.
+  Parameter erasedCores_refl: forall c, erasedCores c c.
+
+  Parameter at_external_erase:
+    forall c c' (Herase: erasedCores c c'),
+      match at_external Sem c, at_external Sem c' with
+      | Some (ef, sig, vs), Some (ef', sig', vs') =>
+        ef = ef' /\ sig = sig' /\ erased_val_list vs vs'
+      | None, None => True
+      | _, _ => False
+      end.
+
+  Parameter after_external_erase:
+    forall v v' c c' c2
+      (HeraseCores: erasedCores c c')
+      (HeraseVal: erased_val v v')
+      (Hafter_external: after_external SEM.Sem (Some v) c = Some c2),
+    exists c2',
+      after_external SEM.Sem (Some v') c' = Some c2' /\
+      erasedCores c2 c2'.
+  
+  Parameter erasure_initial_core:
+    forall ge v arg v' arg' c
+      (Hv: erased_val v v')
+      (Harg: erased_val arg arg')
+      (Hinit: initial_core Sem ge v [:: arg] = Some c),
+      initial_core Sem ge v' [:: arg'] = Some c.
+  
+  Parameter halted_erase:
+    forall c c'
+      (HeraseCores: erasedCores c c')
+      (Hhalted: halted SEM.Sem c),
+      halted SEM.Sem c'.
+
+  Parameter evstep_erase:
+    forall ge c1 c1' c2 ev m1 m1' m2
+      (HeraseCores: erasedCores c1 c1')
+      (HerasedMem: erasedMem m1 m1')
+      (Hstep: ev_step Sem ge c1 m1 ev c2 m2),
+    exists c2' m2',
+      ev_step Sem ge c1' m1' ev c2' m2' /\
+      erasedCores c2 c2' /\ erasedMem m2 (erasePerm m2').
+
+  Hint Resolve erasedCores_refl : erased.
+  
+End CoreErasure.
+
+Module ThreadPoolErasure (SEM: Semantics)
+       (Machines: MachinesSig with Module SEM := SEM)
+       (CE : CoreErasure SEM).
+  Import ValErasure CE
+         Machines DryMachine ThreadPool.
+  
+  Definition erasedCtl c c' : Prop :=
+    match c, c' with
+    | Kinit vf arg, Kinit vf' arg' =>
+      erased_val vf vf' /\ erased_val arg arg'
+    | Krun c, Krun c' =>
+      erasedCores c c'
+    | Kblocked c, Kblocked c' =>
+      erasedCores c c'
+    | Kresume c arg, Kresume c' arg' =>
+      erasedCores c c' /\ arg = arg'
+    (*we don't use this and our semantics are strange*)
+    | _, _  => False
+    end.
+
+  Inductive erased_threadPool tp (tp' : ErasedMachine.ThreadPool.t) :=
+  | ErasedPool :
+      num_threads tp = ErasedMachine.ThreadPool.num_threads tp' ->
+      (forall i (cnti: containsThread tp i)
+         (cnti': ErasedMachine.ThreadPool.containsThread tp' i),
+          erasedCtl (getThreadC cnti)
+                    (ErasedMachine.ThreadPool.getThreadC cnti')) ->
+      erased_threadPool tp tp'.
+
+  Lemma erasedPool_contains:
+    forall tp1 tp1' 
+      (HerasedPool: erased_threadPool tp1 tp1') i,
+      containsThread tp1 i <-> ErasedMachine.ThreadPool.containsThread tp1' i.
+  Proof.
+    intros.
+    inversion HerasedPool.
+    unfold containsThread, ErasedMachine.ThreadPool.containsThread.
+    rewrite H.
+    split; auto.
+  Qed.
+
+  Lemma erasedCtl_refl:
+    forall c, erasedCtl c c.
+  Proof with eauto with erased.
+    destruct c; simpl...
+  Qed.
+  
+  Lemma erased_updLockSet:
+    forall tp tp' addr addr' rmap rmap',
+      erased_threadPool tp tp' ->
+      erased_threadPool (updLockSet tp addr rmap)
+                        (ErasedMachine.ThreadPool.updLockSet tp' addr' rmap').
+  Proof.
+    intros.
+    inversion H.
+    constructor; auto.
+  Qed.
+  
+  Lemma erased_updThread:
+    forall tp tp' i (cnti: containsThread tp i)
+      (cnti': ErasedMachine.ThreadPool.containsThread tp' i) c c' pmap pmap',
+      erased_threadPool tp tp' ->
+      erasedCtl c c' ->
+      erased_threadPool (updThread cnti c pmap)
+                        (ErasedMachine.ThreadPool.updThread cnti' c' pmap').
+  Proof.
+    intros.
+    inversion H.
+    constructor; auto.
+    intros.
+    destruct (i0 == i) eqn:Heq; move/eqP:Heq=>Heq.
+    subst. rewrite gssThreadCode.
+    rewrite ErasedMachine.ThreadPool.gssThreadCode; auto.
+    rewrite gsoThreadCode; auto.
+    rewrite ErasedMachine.ThreadPool.gsoThreadCode; auto.
+  Qed.
+
+  Lemma erased_addThread:
+    forall tp tp' i (cnti: containsThread tp i)
+      (cnti': ErasedMachine.ThreadPool.containsThread tp' i) v arg v' arg' pmap pmap',
+      erased_threadPool tp tp' ->
+      erased_val v v' ->
+      erased_val arg arg' ->
+      erased_threadPool (addThread tp v arg pmap)
+                        (ErasedMachine.ThreadPool.addThread tp' v arg pmap').
+  Proof with eauto with erased.
+    intros.
+    inversion H.
+    constructor.
+    unfold addThread, ErasedMachine.ThreadPool.addThread; simpl. rewrite H2; auto.
+    intros.
+    assert (cnti00 := cntAdd' _ _ _  cnti0).
+    assert (cnti0'0 := ErasedMachine.ThreadPool.cntAdd' _ _ _  cnti'0).
+    destruct cnti00 as [[cnti00 ?] | Heq];
+      destruct cnti0'0 as [[cnti0'0 ?] | ?].
+    - erewrite gsoAddCode with (cntj := cnti00) by eauto.
+      erewrite ErasedMachine.ThreadPool.gsoAddCode with (cntj := cnti0'0) by eauto.
+      eauto.
+    - exfalso; subst; apply H4.
+      destruct (num_threads tp), (ErasedMachine.ThreadPool.num_threads tp');
+        simpl; inversion H2; auto.
+    - exfalso; subst; apply H4.
+      destruct (num_threads tp), (ErasedMachine.ThreadPool.num_threads tp');
+        simpl; inversion H2; auto.
+    - subst. erewrite gssAddCode by eauto.
+      erewrite ErasedMachine.ThreadPool.gssAddCode; eauto.
+      simpl...
+  Qed.
+  
+  Lemma erased_remLockSet:
+    forall tp tp' addr addr',
+      erased_threadPool tp tp' ->
+      erased_threadPool (remLockSet tp addr)
+                        (ErasedMachine.ThreadPool.remLockSet tp' addr').
+  Proof.
+    intros.
+    inversion H.
+    constructor; auto.
+  Qed.
+
+  Hint Resolve erased_updLockSet erased_updThread
+       erased_addThread erased_remLockSet: erased.
+
+End ThreadPoolErasure.
+  
+(** ** Erasure from FineConc to SC*)
+Module SCErasure (SEM: Semantics)
+       (Machines: MachinesSig with Module SEM := SEM)
+       (AsmContext: AsmContext SEM Machines)
+       (CE : CoreErasure SEM).
+  Module ThreadPoolErasure := ThreadPoolErasure SEM Machines CE.
+  Import ValErasure MemErasure CE ThreadPoolErasure.
+  Import Machines DryMachine ThreadPool AsmContext.
+
+  Import event_semantics.
+  (** ** Simulation for syncStep, startStep, resumeStep, suspendStep,
+  and haltedStep *)
+  
+  Lemma syncStep_erase:
+    forall ge tp1 tp1' m1 m1' tp2 m2 i ev
+      (HerasePool: erased_threadPool tp1 tp1')
+      (cnti: containsThread tp1 i)
+      (cnti': ErasedMachine.ThreadPool.containsThread tp1' i)
+      (HerasedMem: erasedMem m1 m1')
+      (Hcomp1: mem_compatible tp1 m1)
+      (Hcomp1': ErasedMachine.mem_compatible tp1' m1')
+      (Hstep: syncStep ge cnti Hcomp1 tp2 m2 ev),
+    exists tp2' m2',
+      ErasedMachine.syncStep ge cnti' Hcomp1' tp2' m2' ev /\
+      erased_threadPool tp2 tp2' /\ erasedMem m2 m2'.
+  Proof with eauto with erased.
+    intros.
+    inversion HerasePool as [Hnum Hthreads].
+    specialize (Hthreads _ cnti cnti').      
+    inversion Hstep; subst;
+    match goal with
+    | [H: erasedCtl ?Expr1 ?Expr2, H1: ?Expr1 = _ |- _] =>
+      rewrite H1 in H; simpl in H;
+      destruct Expr2 eqn:?
+    end; try (by exfalso);
+    try match goal with
+        | [H: Mem.load _ _ _ _ = Some _ |- _] =>
+          eapply mem_load_erased in H; eauto
+        end;
+    try match goal with
+        | [H: Mem.store _ _ _ _ _ = Some _ |- _] =>
+          eapply mem_store_erased in H; eauto;
+          destruct Hstore as [m2' [Hstore HerasedMem']]
+        end;
+    try match goal with
+        | [|- _ <> Vundef] => intro Hcontra; discriminate
+        end;
+    match goal with
+    | [H: at_external _ _ = _, H1: erasedCores _ _ |- _] =>
+      pose proof (at_external_erase H1);
+        match goal with
+        | [H2: match at_external _ _ with _ => _ end |- _] =>
+          rewrite H in H2;
+            match goal with
+            | [H3: match at_external ?E1 ?E2 with _ => _ end |- _] =>
+              destruct (at_external E1 E2) as [[[? ?] ?]|] eqn:?; try by exfalso
+            end
+        end
+    end;
+    repeat match goal with
+           | [H: _ /\ _ |- _] => destruct H
+           | [H: erased_val_list _ _ |- _] =>
+             inv H
+           | [H: erased_val (Vptr _ _) _ |- _] => inv H
+           end; subst.
+    - exists (ErasedMachine.ThreadPool.updThreadC cnti' (Kresume c0 Vundef)), m2'.
+      split; [econstructor; eauto | split; eauto].
+      constructor. simpl; eauto.
+      intros j cntj cntj'.
+      rewrite gLockSetCode.
+      destruct (i == j) eqn:Hij; move/eqP:Hij=>Hij.
+      + subst.
+        rewrite gssThreadCode.
+        rewrite ErasedMachine.ThreadPool.gssThreadCC.
+        simpl; auto.
+      + rewrite gsoThreadCode; auto.
+        assert (cntj0' := ErasedMachine.ThreadPool.cntUpdateC' _ _ cntj').
+        erewrite <- @ErasedMachine.ThreadPool.gsoThreadCC with (cntj := cntj0')
+          by eauto.
+        inversion HerasePool; eauto.
+    - exists (ErasedMachine.ThreadPool.updThreadC cnti' (Kresume c0 Vundef)), m2'.
+      split; [econstructor; eauto | split; eauto].
+      constructor. simpl; eauto.
+      intros j cntj cntj'.
+      rewrite gLockSetCode.
+      destruct (i == j) eqn:Hij; move/eqP:Hij=>Hij.
+      + subst.
+        rewrite gssThreadCode.
+        rewrite ErasedMachine.ThreadPool.gssThreadCC.
+        simpl; auto.
+      + rewrite gsoThreadCode; auto.
+        assert (cntj0' := ErasedMachine.ThreadPool.cntUpdateC' _ _ cntj').
+        erewrite <- @ErasedMachine.ThreadPool.gsoThreadCC with (cntj := cntj0')
+          by eauto.
+        inversion HerasePool; eauto.
+    - exists (ErasedMachine.ThreadPool.addThread
+           (ErasedMachine.ThreadPool.updThreadC cnti' (Kresume c0 Vundef))
+           (Vptr b ofs) v'0 tt), m1'.
+      split; [econstructor; eauto | split; eauto].
+      constructor. simpl; eauto. rewrite Hnum. auto.
+      intros j cntj cntj'.
+      assert (cntj0 := cntAdd' _ _ _ cntj).
+      destruct cntj0 as [[cntj0 ?] | Heq].
+      + (* case it's an old thread*)
+        erewrite @gsoAddCode with (cntj := cntj0) by eauto.
+        assert (cntj00 := cntUpdate' _ _ _ cntj0).
+        assert (cntj00': ErasedMachine.ThreadPool.containsThread tp1' j)
+          by (unfold containsThread,ErasedMachine.ThreadPool.containsThread;
+               rewrite <- Hnum; auto).
+        assert (cntj0' := ErasedMachine.ThreadPool.cntUpdateC (Kresume c0 Vundef)
+                                                              cnti' cntj00').
+        erewrite @ErasedMachine.ThreadPool.gsoAddCode with (cntj := cntj0')
+          by eauto.
+        destruct (i == j) eqn:Hij; move/eqP:Hij=>Hij.
+        * subst.
+          rewrite gssThreadCode.
+          rewrite ErasedMachine.ThreadPool.gssThreadCC.
+          simpl; auto.
+        * rewrite gsoThreadCode; auto.
+          erewrite <- @ErasedMachine.ThreadPool.gsoThreadCC with (cntj := cntj00')
+            by eauto.
+          inversion HerasePool; eauto.
+      + (*case j is the just addded thread *)
+        subst.
+        erewrite gssAddCode by (unfold latestThread; reflexivity).
+        erewrite ErasedMachine.ThreadPool.gssAddCode
+          by (unfold ErasedMachine.ThreadPool.latestThread;
+               simpl; rewrite Hnum; auto).
+        simpl; auto.
+    - exists (ErasedMachine.ThreadPool.updThreadC cnti' (Kresume c0 Vundef)), m2'.
+      split; [econstructor; eauto | split; eauto].
+      constructor. simpl; eauto.
+      intros j cntj cntj'.
+      rewrite gLockSetCode.
+      destruct (i == j) eqn:Hij; move/eqP:Hij=>Hij.
+      + subst.
+        rewrite gssThreadCode.
+        rewrite ErasedMachine.ThreadPool.gssThreadCC.
+        simpl; auto.
+      + rewrite gsoThreadCode; auto.
+        assert (cntj0' := ErasedMachine.ThreadPool.cntUpdateC' _ _ cntj').
+        erewrite <- @ErasedMachine.ThreadPool.gsoThreadCC with (cntj := cntj0')
+          by eauto.
+        inversion HerasePool; eauto.
+    - exists (ErasedMachine.ThreadPool.updThreadC cnti' (Kresume c0 Vundef)), m1'.
+      split; [econstructor; eauto | split; eauto].
+      constructor. simpl; eauto.
+      intros j cntj cntj'.
+      rewrite gRemLockSetCode.
+      destruct (i == j) eqn:Hij; move/eqP:Hij=>Hij.
+      + subst.
+        rewrite gssThreadCode.
+        rewrite ErasedMachine.ThreadPool.gssThreadCC.
+        simpl; auto.
+      + rewrite gsoThreadCode; auto.
+        assert (cntj0' := ErasedMachine.ThreadPool.cntUpdateC' _ _ cntj').
+        erewrite <- @ErasedMachine.ThreadPool.gsoThreadCC with (cntj := cntj0')
+          by eauto.
+        inversion HerasePool; eauto.
+    - exists tp1', m1'.
+      split; [econstructor; eauto | split; eauto].
+  Qed.
+
+  (*TODO: move that in asm_context module and see if it works*)
+ Ltac pf_cleanup :=
+    repeat match goal with
+           | [H1: invariant ?X, H2: invariant ?X |- _] =>
+             assert (H1 = H2) by (by eapply proof_irr);
+               subst H2
+           | [H1: mem_compatible ?TP ?M, H2: mem_compatible ?TP ?M |- _] =>
+             assert (H1 = H2) by (by eapply proof_irr);
+               subst H2
+           | [H1: is_true (leq ?X ?Y), H2: is_true (leq ?X ?Y) |- _] =>
+             assert (H1 = H2) by (by eapply proof_irr); subst H2
+           | [H1: containsThread ?TP ?M, H2: containsThread ?TP ?M |- _] =>
+             assert (H1 = H2) by (by eapply proof_irr); subst H2
+           | [H1: containsThread ?TP ?M,
+                  H2: containsThread (@updThreadC _ ?TP _ _) ?M |- _] =>
+             apply cntUpdateC' in H2;
+               assert (H1 = H2) by (by eapply cnt_irr); subst H2
+           | [H1: containsThread ?TP ?M,
+                  H2: containsThread (@updThread _ ?TP _ _ _) ?M |- _] =>
+             apply cntUpdate' in H2;
+               assert (H1 = H2) by (by eapply cnt_irr); subst H2
+           end.
+  
+  Lemma startStep_erasure:
+    forall ge tp1 tp1' tp2 i
+      (HerasePool: erased_threadPool tp1 tp1')
+      (cnti: containsThread tp1 i)
+      (cnti': ErasedMachine.ThreadPool.containsThread tp1' i)
+      (Hstep: FineConc.start_thread ge cnti tp2),
+    exists tp2',
+      SC.start_thread ge cnti' tp2' /\
+      erased_threadPool tp2 tp2'.
+  Proof.
+    intros.
+    inversion HerasePool as [Hnum Hthreads].
+    specialize (Hthreads _ cnti cnti').
+    inversion Hstep; subst.
+    pf_cleanup;
+      match goal with
+        [H: erasedCtl ?Expr1 ?Expr2, H1: ?Expr1 = _ |- _] =>
+        rewrite H1 in H; simpl in H;
+        destruct Expr2 eqn:?
+      end; try (by exfalso).
+    repeat match goal with
+           | [H: _ /\ _ |- _] => destruct H
+           | [H: erased_val_list _ _ |- _] =>
+             inv H
+           | [H: erased_val (Vptr _ _) _ |- _] => inv H
+           end; subst.
+    eapply erasure_initial_core in Hinitial; eauto.
+    exists (ErasedMachine.ThreadPool.updThreadC cnti' (Krun c_new)).
+    split; econstructor; eauto.
+    unfold ErasedMachine.invariant; auto.
+    intros j cntj cntj'.
+    destruct (i == j) eqn:Hij; move/eqP:Hij=>Hij.
+    + subst.
+      rewrite gssThreadCC.
+      rewrite ErasedMachine.ThreadPool.gssThreadCC.
+      simpl. apply erasedCores_refl.
+    +
+      assert (cntj0' := ErasedMachine.ThreadPool.cntUpdateC' _ _ cntj').
+      assert (cntj0 := cntUpdateC' _ _ cntj).
+      erewrite <- @gsoThreadCC with (cntj :=  cntj0) by eauto.
+      erewrite <- @ErasedMachine.ThreadPool.gsoThreadCC with (cntj := cntj0')
+        by eauto.
+      inversion HerasePool; eauto.
+  Qed.
+
+  Lemma resumeStep_erasure:
+    forall tp1 tp1' tp2 i
+      (HerasePool: erased_threadPool tp1 tp1')
+      (cnti: containsThread tp1 i)
+      (cnti': ErasedMachine.ThreadPool.containsThread tp1' i)
+      (Hstep: FineConc.resume_thread cnti tp2),
+    exists tp2',
+      SC.resume_thread cnti' tp2' /\
+      erased_threadPool tp2 tp2'.
+  Proof.
+    intros.
+    inversion HerasePool as [Hnum Hthreads].
+    specialize (Hthreads _ cnti cnti').
+    inversion Hstep; subst.
+    pf_cleanup;
+      match goal with
+        [H: erasedCtl ?Expr1 ?Expr2, H1: ?Expr1 = _ |- _] =>
+        rewrite H1 in H; simpl in H;
+        destruct Expr2 eqn:?
+      end; try (by exfalso).
+    destruct Hthreads as [HeraseCores Heq]. subst v.
+    pose proof (at_external_erase HeraseCores).
+    rewrite Hat_external in H.
+    destruct X, p.
+    destruct (at_external SEM.Sem c0) eqn:Hat_external'; try by exfalso.
+    destruct p as [[? ?] ?].
+    destruct H as [? [? ?]]; subst.
+    eapply after_external_erase with (v' := Vint Int.zero) in Hafter_external;
+      eauto with erased.
+    destruct Hafter_external as [c2' [Hafter_external' HerasedCores']].
+    exists (ErasedMachine.ThreadPool.updThreadC cnti' (Krun c2')).
+    split.
+    eapply SC.ResumeThread with (c := c0); simpl in *; eauto.
+    unfold ErasedMachine.invariant; auto.
+    constructor.
+    simpl. auto.
+    intros j cntj cntj'.
+    destruct (i == j) eqn:Hij; move/eqP:Hij=>Hij.
+    + subst.
+      rewrite gssThreadCC.
+      rewrite ErasedMachine.ThreadPool.gssThreadCC.
+      simpl; eauto.
+    +
+      assert (cntj0' := ErasedMachine.ThreadPool.cntUpdateC' _ _ cntj').
+      assert (cntj0 := cntUpdateC' _ _ cntj).
+      erewrite <- @gsoThreadCC with (cntj :=  cntj0) by eauto.
+      erewrite <- @ErasedMachine.ThreadPool.gsoThreadCC with (cntj := cntj0')
+        by eauto.
+      inversion HerasePool; eauto.
+  Qed.
+  
+  Lemma suspendStep_erasure:
+    forall tp1 tp1' tp2 i
+      (HerasePool: erased_threadPool tp1 tp1')
+      (cnti: containsThread tp1 i)
+      (cnti': ErasedMachine.ThreadPool.containsThread tp1' i)
+      (Hstep: FineConc.suspend_thread cnti tp2),
+    exists tp2',
+      SC.suspend_thread cnti' tp2' /\
+      erased_threadPool tp2 tp2'.
+  Proof.
+    intros.
+    inversion HerasePool as [Hnum Hthreads].
+    specialize (Hthreads _ cnti cnti').
+    inversion Hstep; subst.
+    pf_cleanup;
+      match goal with
+        [H: erasedCtl ?Expr1 ?Expr2, H1: ?Expr1 = _ |- _] =>
+        rewrite H1 in H; simpl in H;
+        destruct Expr2 eqn:?
+      end; try (by exfalso).
+    pose proof (at_external_erase Hthreads).
+    rewrite Hat_external in H.
+    destruct X, p.
+    destruct (at_external SEM.Sem c0) eqn:Hat_external'; try by exfalso.
+    destruct p as [[? ?] ?].
+    destruct H as [? [? ?]]; subst.
+    exists (ErasedMachine.ThreadPool.updThreadC cnti' (Kblocked c0)).
+    split.
+    eapply SC.SuspendThread with (c := c0); simpl in *; eauto.
+    unfold ErasedMachine.invariant; auto.
+    constructor.
+    simpl. auto.
+    intros j cntj cntj'.
+    destruct (i == j) eqn:Hij; move/eqP:Hij=>Hij.
+    + subst.
+      rewrite gssThreadCC.
+      rewrite ErasedMachine.ThreadPool.gssThreadCC.
+      simpl; eauto.
+    +
+      assert (cntj0' := ErasedMachine.ThreadPool.cntUpdateC' _ _ cntj').
+      assert (cntj0 := cntUpdateC' _ _ cntj).
+      erewrite <- @gsoThreadCC with (cntj :=  cntj0) by eauto.
+      erewrite <- @ErasedMachine.ThreadPool.gsoThreadCC with (cntj := cntj0')
+        by eauto.
+      inversion HerasePool; eauto.
+  Qed.
+
+  Lemma haltStep_erasure:
+    forall tp1 tp1' i
+      (HerasePool: erased_threadPool tp1 tp1')
+      (cnti: containsThread tp1 i)
+      (cnti': ErasedMachine.ThreadPool.containsThread tp1' i)
+      (Hstep: threadHalted cnti),
+      ErasedMachine.threadHalted cnti'.
+  Proof.
+    intros.
+    inversion HerasePool as [Hnum Hthreads].
+    specialize (Hthreads _ cnti cnti').
+    inversion Hstep; subst.
+    pf_cleanup.
+    rewrite Hcode in Hthreads.
+    simpl in Hthreads.
+    destruct (ErasedMachine.ThreadPool.getThreadC cnti') eqn:?;
+             try by exfalso.
+    assert (halted SEM.Sem c0)
+      by (eapply halted_erase; eauto).
+    econstructor; eauto.
+  Qed.
+
+   Lemma threadStep_erase:
+    forall ge tp1 tp1' m1 m1' tp2 m2 i ev
+      (HerasePool: erased_threadPool tp1 tp1')
+      (cnti: containsThread tp1 i)
+      (cnti': ErasedMachine.ThreadPool.containsThread tp1' i)
+      (HerasedMem: erasedMem m1 m1')
+      (Hcomp1: mem_compatible tp1 m1)
+      (Hcomp1': ErasedMachine.mem_compatible tp1' m1')
+      (Hstep: threadStep ge cnti Hcomp1 tp2 m2 ev),
+    exists tp2' m2',
+      ErasedMachine.threadStep ge cnti' Hcomp1' tp2' m2' ev /\
+      erased_threadPool tp2 tp2' /\ erasedMem m2 (erasePerm m2').
+  Proof.
+    intros.
+    inversion HerasePool as [Hnum Hthreads].
+    specialize (Hthreads _ cnti cnti').
+    inversion Hstep; subst.
+    pf_cleanup;
+      match goal with
+        [H: erasedCtl ?Expr1 ?Expr2, H1: ?Expr1 = _ |- _] =>
+        rewrite H1 in H; simpl in H;
+        destruct Expr2 eqn:?
+      end; try (by exfalso).
+    eapply erasedMem_restr with (Hlt := Hcomp1 i cnti) in HerasedMem.
+    eapply evstep_erase in Hcorestep; eauto.
+    destruct Hcorestep as (c2' & m2' & Hevstep' & HerasedCores' & HerasedMem').
+    exists (ErasedMachine.ThreadPool.updThreadC cnti' (Krun c2')), m2'.
+    split; eauto.
+    econstructor; eauto.
+    split; eauto.
+    constructor; eauto.
+    intros j cntj cntj'.
+    destruct (i == j) eqn:Hij; move/eqP:Hij=>Hij.
+    + subst.
+      rewrite gssThreadCode.
+      rewrite ErasedMachine.ThreadPool.gssThreadCC.
+      simpl; eauto.
+    +
+      assert (cntj0' := ErasedMachine.ThreadPool.cntUpdateC' _ _ cntj').
+      assert (cntj0 := cntUpdate' _ _ _ cntj).
+      erewrite  @gsoThreadCode with (cntj :=  cntj0) by eauto.
+      erewrite <- @ErasedMachine.ThreadPool.gsoThreadCC with (cntj := cntj0')
+        by eauto.
+      inversion HerasePool; eauto.
+  Qed.
+
+  Notation fstep := (corestep fine_semantics).
+  Notation scstep := (corestep sc_semantics).
+
+  (** A step on the FineConc machine can be matched by a step on the
+  SC machine producing the same event *)
+  Lemma sc_sim:
+    forall ge tp1 tp1' i U tr tr' m1 m1' tp2 m2
+      (HerasePool: erased_threadPool tp1 tp1')
+      (HerasedMem: erasedMem m1 m1')
+      (Hfstep: fstep ge (i :: U, tr, tp1) m1 (U, tr', tp2) m2),
+    exists tp2' m2',
+      scstep ge (i :: U, tr, tp1') m1' (U, tr', tp2') m2' /\
+      erased_threadPool tp2 tp2' /\ erasedMem m2 m2'.
+  Proof.
+    intros.
+    inversion Hfstep; simpl in *; subst;
+    inv HschedN;
+    try match goal with
+        | [H: containsThread _ ?I |- _ ] =>
+          assert (ErasedMachine.ThreadPool.containsThread tp1' I)
+            by (eapply erasedPool_contains; eauto)
+        end;
+    assert (Hcomp1' : ErasedMachine.mem_compatible tp1' m1')
+      by (unfold ErasedMachine.mem_compatible; auto).
+    - assert (Hstep' := startStep_erasure HerasePool H Htstep).
+      destruct Hstep' as [tp2' [Hstart' HerasePool']].
+      exists tp2', m1'.
+      split. econstructor 1; simpl; eauto.
+      split; eauto.
+    - assert (Hstep' := resumeStep_erasure HerasePool H Htstep).
+      destruct Hstep' as [tp2' [Hstart' HerasePool']].
+      exists tp2', m1'.
+      split. econstructor 2; simpl; eauto.
+      split; eauto.
+    - assert (Htstep' := threadStep_erase HerasePool H HerasedMem Hcomp1' Htstep).
+      destruct Htstep' as [tp2' [m2' [Htstep' [HerasePool' HerasedMem']]]].
+      exists tp2', (erasePerm m2').
+      split.
+      eapply SC.thread_step; eauto.
+      split; eauto.
+      eapply erasedMem_dilute_1; eauto.
+    - assert (Hstep' := suspendStep_erasure HerasePool H Htstep).
+      destruct Hstep' as [tp2' [Hstart' HerasePool']].
+      exists tp2', m1'.
+      split. econstructor 4; simpl; eauto.
+      split; eauto.
+    - assert (Hstep' := syncStep_erase HerasePool H HerasedMem Hcomp1' Htstep).
+      destruct Hstep' as [tp2' [m2' [Hstep' [HerasePool' HerasedMem']]]].
+      exists tp2', m2'.
+      split.
+      eapply SC.sync_step; eauto.
+      split; eauto.
+    - eapply haltStep_erasure with (cnti' := H) in Hhalted; eauto.
+      exists tp1', m1';
+        split; eauto.
+      econstructor 6; simpl; eauto.
+    - assert (~ ErasedMachine.ThreadPool.containsThread tp1' tid).
+      { intros Hcontra.
+        destruct HerasePool as [Hnum _].
+        unfold containsThread, ErasedMachine.ThreadPool.containsThread in *.
+        rewrite <- Hnum in Hcontra.
+        auto.
+      }
+      exists tp1', m1'.
+      split.
+      econstructor 7; simpl; eauto.
+      split; eauto.
+  Qed.
+  
+  Notation sc_safe := (SC.fsafe the_ge).
+  Notation fsafe := (FineConc.fsafe the_ge).
+
+  Inductive sc_execution :
+    SC.MachState -> mem -> SC.MachState -> mem -> Prop :=
+  | refl_sc_exec : forall ms (m : mem),
+      SC.halted ms ->
+      sc_execution ms m ms m
+  | step_sc_trans : forall i U U'
+                      (tp tp' tp'': SC.machine_state)
+                      (tr tr' tr'': SC.event_trace)
+                      (m m' m'' : mem),
+      SC.MachStep the_ge (i :: U, tr, tp) m (U, tr', tp') m' ->
+      sc_execution (U, tr', tp') m' (U', tr'', tp'') m'' ->
+      sc_execution (i :: U,tr,tp) m (U',tr'',tp'') m''.
+
+  Inductive fine_execution :
+    FineConc.MachState -> mem -> FineConc.MachState -> mem -> Prop :=
+  | refl_fine_exec : forall ms (m : mem),
+      FineConc.halted ms ->
+      fine_execution ms m ms m
+  | step_fine_trans : forall i U U'
+                        (tp tp' tp'': FineConc.machine_state)
+                        (tr tr' tr'': FineConc.event_trace)
+                        (m m' m'' : mem),
+      FineConc.MachStep the_ge (i :: U, tr, tp) m (U, tr ++ tr', tp') m' ->
+      fine_execution (U, tr ++ tr', tp') m' (U', tr ++ tr' ++ tr'', tp'') m'' ->
+      fine_execution (i :: U,tr,tp) m (U',tr ++ tr' ++ tr'',tp'') m''.
+
+  (* TODO: Move this lemma. Maybe definitions above it too*)
+  Lemma fstep_trace_irr:
+    forall U i tp m tp' m' tr tr'
+      (Hstep: FineConc.MachStep the_ge (i :: U, tr, tp) m (U, tr', tp') m'),
+    forall tr'', exists ev,
+        FineConc.MachStep the_ge (i :: U, tr'', tp) m (U, tr'' ++ ev, tp') m'.
+  Proof.
+    intros.
+    inversion Hstep; subst; simpl in *; subst; inv HschedN; pf_cleanup.
+    - exists [::]; erewrite cats0; econstructor; simpl; eauto.
+    - exists [::]; erewrite cats0; econstructor 2; simpl; eauto.
+    - exists (map [eta Events.internal tid] ev); econstructor 3; simpl; eauto.
+    - exists [::]; erewrite cats0; econstructor 4; simpl; eauto.
+    - exists [:: Events.external tid ev]; econstructor 5; simpl; eauto.
+    - exists [::]; erewrite cats0; econstructor 6; simpl; eauto.
+    - exists [::]; erewrite cats0; econstructor 7; simpl; eauto.
+  Qed.
+
+  Lemma fsafe_execution:
+    forall tpf mf U tr,
+      fsafe tpf mf U (size U).+1 ->
+      exists tpf' mf' tr',
+        fine_execution (U, tr, tpf) mf ([::], tr ++ tr', tpf') mf'.
+  Proof.
+    intros.
+    generalize dependent mf.
+    generalize dependent tpf.
+    generalize dependent tr.
+    induction U; intros.
+    do 2 eexists. exists [::].
+    erewrite cats0.
+    econstructor 1; eauto.
+    simpl in *.
+    inversion H; subst.
+    simpl in H0; by exfalso.
+    simpl in *.
+    assert (exists ev,
+               FineConc.MachStep the_ge ((a :: U), tr, tpf) mf
+                                 (U, tr ++ ev, tp') m')
+      by (eapply fstep_trace_irr; eauto).
+    destruct H0 as [ev Hstep].
+    specialize (IHU (tr ++ ev) _ _ H2).
+    destruct IHU as (tpf'' & mf'' & tr'' & Hexec).
+    rewrite <- catA in Hexec.
+    exists tpf'', mf'', (ev ++ tr'').
+    econstructor 2; eauto.
+  Qed.
+
+  (** The initial state of the SC machine is an erasure of the initial
+  state of the FineConc machine*)
+ Lemma init_erasure:
+    forall f arg U tpsc tpf
+      (HinitSC: sc_init f arg = Some (U, [::], tpsc))
+      (HinitF: tpf_init f arg = Some (U, [::], tpf)),
+      erased_threadPool tpf tpsc.
+  Proof.
+    intros.
+    unfold sc_init, tpf_init in *.
+    simpl in *. unfold SC.init_machine, FineConc.init_machine in *.
+    unfold init_mach, ErasedMachine.init_mach in *.
+    simpl in *.
+    destruct (initial_core SEM.Sem the_ge f arg); try discriminate.
+    destruct init_perm; try discriminate.
+    inv HinitSC. inv HinitF.
+    unfold initial_machine, ErasedMachine.initial_machine.
+    simpl.
+    econstructor. simpl; eauto.
+    intros. 
+    simpl.
+    apply erasedCores_refl; auto.
+  Qed.
+
+  (** Any execution of the FineConc machine resulting in some trace
+    tr' can be matched by an execution of the SC machine with the
+    same trace*)
+  Lemma execution_sim:
+    forall U U' tpf tpf' mf mf' tpsc msc tr tr' 
+      (Hexec: fine_execution (U, tr, tpf) mf (U', tr', tpf') mf')
+      (HerasedPool: erased_threadPool tpf tpsc)
+      (HerasedMem: erasedMem mf msc),
+    exists tpsc' msc',
+      sc_execution (U, tr, tpsc) msc (U', tr', tpsc') msc' /\
+      erased_threadPool tpf' tpsc' /\ erasedMem mf' msc'.
+  Proof.
+    intros U.
+    induction U.
+    - intros.
+      inversion Hexec; subst.
+      exists tpsc, msc.
+      split.
+      econstructor 1. simpl; auto.
+      split; auto.
+    - intros.
+      inversion Hexec; subst.
+      + simpl in H5; by exfalso.
+      + eapply sc_sim in H8; eauto.
+        destruct H8 as (tpsc0 & msc0 & Hstep0 & HerasedPool0 & HerasedMem0).
+        specialize (IHU _ _ _ _ _ _ _ _ _ H9 HerasedPool0 HerasedMem0).
+        destruct IHU as (tpsc2' & msc2' & Hsexec & HerasedPool' & HerasedMem').
+        exists tpsc2', msc2'.
+        split; eauto.
+        econstructor; eauto.
+  Qed.
+
+  (** Safety of the SC machine*)
+  Lemma fsafe_implies_scsafe:
+    forall sched tpsc tpf mf msc
+      (Hsafe: fsafe tpf mf sched (size sched).+1)
+      (HerasedPool: erased_threadPool tpf tpsc)
+      (HerasedMem: erasedMem mf msc),
+      sc_safe tpsc msc sched (size sched).+1.
+  Proof.
+    intro sched.
+    induction sched as [|i sched]; intros.
+    - simpl in *. inversion Hsafe;
+        eapply SC.HaltedSafe with (tr := tr);
+        simpl; auto.
+    - simpl in Hsafe.
+      inversion Hsafe; subst.
+      simpl in H; by exfalso.
+      simpl in *.
+      eapply sc_sim in H0; eauto.
+      destruct H0 as (tpsc2' & msc2' & Hstep & HerasedPool' & HerasedMem').
+      econstructor 3; eauto.
+  Qed.
+  
+  Theorem sc_erasure:
+    forall sched f arg U tpsc tpf m
+      (Hmem: init_mem = Some m)
+      (HinitSC: sc_init f arg = Some (U, [::], tpsc))
+      (HinitF: tpf_init f arg = Some (U, [::], tpf))
+      (HsafeF: fsafe tpf (DryMachine.diluteMem m) sched (size sched).+1),
+      sc_safe tpsc (ErasedMachine.diluteMem m) sched (size sched).+1 /\
+      (forall tpf' mf' tr,
+          fine_execution (sched, [::], tpf) (DryMachine.diluteMem m)
+                         ([::], tr, tpf') mf' ->
+          exists tpsc' msc',
+            sc_execution (sched, [::], tpsc) (ErasedMachine.diluteMem m)
+                         ([::], tr, tpsc') msc' /\
+            erased_threadPool tpf' tpsc' /\ erasedMem mf' msc').
+  Proof.
+    intros.
+    assert (HpoolErase := init_erasure _ _ HinitSC HinitF).
+    assert (HmemErase : erasedMem (diluteMem m) (ErasedMachine.diluteMem m)).
+    { econstructor; eauto.
+      intros.
+      assert (Hvalid: Mem.valid_block m b)
+        by (unfold Mem.valid_block, ErasedMachine.diluteMem, erasePerm in *;
+             simpl in *; auto).
+      assert (Hperm:= erasePerm_V ofs k Hvalid).
+      unfold permission_at in Hperm; auto.
+    }
+    split; first by (eapply fsafe_implies_scsafe; eauto).
+    intros.
+    eapply execution_sim; eauto.
+  Qed.
+
+End SCErasure.
+  
+  
+
+
+
