concurrency/memory_lemmas.v
@@ -1,0 +1,179 @@
+Require Import compcert.common.Memory.
+Require Import concurrency.permissions.
+Require Import Coq.ZArith.ZArith.
+Require Import compcert.lib.Coqlib.
+
+(** ** Various results about CompCert's memory model*)
+Module MemoryLemmas.
+
+  Global Notation "a # b" := (Maps.PMap.get b a) (at level 1).
+  Transparent Mem.store.
+  (*TODO: see if we can reuse that for gsoMem_obs_eq.*)
+  (*TODO: maybe we don't need to open up the interface here*)
+  Lemma store_contents_other:
+    forall m m' b b' ofs ofs' v chunk
+      (Hstore: Mem.store chunk m b ofs v = Some m')
+      (Hstable: ~ Mem.perm m b' ofs' Cur Writable),
+      Maps.ZMap.get ofs' (Mem.mem_contents m') # b' =
+      Maps.ZMap.get ofs' (Mem.mem_contents m) # b'.
+  Proof.
+    intros.
+    erewrite Mem.store_mem_contents; eauto.
+    simpl.
+    destruct (Pos.eq_dec b b') as [Heq | Hneq];
+      [| by erewrite Maps.PMap.gso by auto].
+    subst b'.
+    rewrite Maps.PMap.gss.
+    destruct (Z_lt_le_dec ofs' ofs) as [Hlt | Hge].
+    erewrite Mem.setN_outside by (left; auto);
+      by reflexivity.
+    destruct (Z_lt_ge_dec
+                ofs' (ofs + (size_chunk chunk)))
+      as [Hlt | Hge'].
+    (* case the two addresses coincide - contradiction*)
+    apply Mem.store_valid_access_3 in Hstore.
+    unfold Mem.valid_access in Hstore. simpl in Hstore.
+    destruct Hstore as [Hcontra _].
+    unfold Mem.range_perm in Hcontra.
+    specialize (Hcontra ofs' (conj Hge Hlt));
+      by exfalso.
+    erewrite Mem.setN_outside by (right; rewrite size_chunk_conv in Hge';
+                                    by rewrite encode_val_length);
+      by auto.
+  Qed.
+
+  Transparent Mem.alloc.
+  
+  Lemma val_at_alloc_1:
+    forall m m' sz nb b ofs
+      (Halloc: Mem.alloc m 0 sz = (m', nb))
+      (Hvalid: Mem.valid_block m b),
+      Maps.ZMap.get ofs (Maps.PMap.get b (Mem.mem_contents m)) =
+      Maps.ZMap.get ofs (Maps.PMap.get b (Mem.mem_contents m')).
+  Proof.
+    intros.
+    unfold Mem.alloc in Halloc.
+    inv Halloc.
+    simpl.
+    rewrite Maps.PMap.gso; auto.
+    intro; subst. unfold Mem.valid_block in *.
+    eapply Plt_strict; eauto.
+  Qed.
+
+  Lemma val_at_alloc_2:
+    forall m m' sz nb ofs
+      (Halloc: Mem.alloc m 0 sz = (m', nb)),
+      Maps.ZMap.get ofs (Maps.PMap.get nb (Mem.mem_contents m')) = Undef.
+  Proof.
+    intros.
+    unfold Mem.alloc in Halloc.
+    inv Halloc.
+    simpl.
+    rewrite PMap.gss, ZMap.gi.
+    reflexivity.
+  Qed.
+
+  Lemma permission_at_alloc_1:
+    forall m m' sz nb b ofs
+      (Halloc: Mem.alloc m 0 sz = (m', nb))
+      (Hvalid: Mem.valid_block m b),
+      permissions.permission_at m b ofs Cur =
+      permissions.permission_at m' b ofs Cur.
+  Proof.
+    intros.
+    Transparent Mem.alloc.
+    unfold Mem.alloc in Halloc.
+    inv Halloc.
+    unfold permissions.permission_at. simpl.
+    rewrite Maps.PMap.gso; auto.
+    intro; subst. unfold Mem.valid_block in *.
+    eapply Plt_strict; eauto.
+  Qed.
+
+  Lemma permission_at_alloc_2:
+    forall m m' sz nb ofs
+      (Halloc: Mem.alloc m 0 sz = (m', nb))
+      (Hofs: (0 <= ofs < sz)%Z),
+      permissions.permission_at m' nb ofs Cur = Some Freeable.
+  Proof.
+    intros.
+    unfold Mem.alloc in Halloc.
+    inv Halloc.
+    unfold permissions.permission_at. simpl.
+    rewrite Maps.PMap.gss.
+    rewrite threads_lemmas.if_true; auto.
+    destruct (zle 0 ofs), (zlt ofs sz); auto;
+    try omega.
+  Qed.
+
+  Lemma permission_at_alloc_3:
+    forall m m' sz nb ofs
+      (Halloc: Mem.alloc m 0 sz = (m', nb))
+      (Hofs: (ofs < 0 \/ ofs >= sz)%Z),
+      permissions.permission_at m' nb ofs Cur = None.
+  Proof.
+    intros.
+    unfold Mem.alloc in Halloc.
+    inv Halloc.
+    unfold permissions.permission_at. simpl.
+    rewrite Maps.PMap.gss.
+    rewrite threads_lemmas.if_false; auto.
+    apply negb_true_iff.
+    destruct (zle 0 ofs), (zlt ofs sz); auto;
+    omega.
+  Qed.
+
+  Lemma mem_free_contents:
+    forall m m2 sz b
+      (Hfree: Mem.free m b 0 sz = Some m2),
+    forall b' ofs,
+      Maps.ZMap.get ofs (Maps.PMap.get b' (Mem.mem_contents m)) =
+      Maps.ZMap.get ofs (Maps.PMap.get b' (Mem.mem_contents m2)).
+  Proof.
+    intros.
+    apply Mem.free_result in Hfree.
+    subst; unfold Mem.unchecked_free.
+    reflexivity.
+  Qed.
+
+  Lemma mem_store_max:
+    forall chunk b ofs v m m',
+      Mem.store chunk m b ofs v = Some m' ->
+      forall b' ofs',
+        (getMaxPerm m) # b' ofs' = (getMaxPerm m') # b' ofs'.
+  Proof.
+    intros.
+    unfold Mem.store in *.
+    destruct (Mem.valid_access_dec m chunk b ofs Writable); try discriminate.
+    inversion H; subst.
+    do 2 rewrite getMaxPerm_correct.
+    reflexivity.
+  Qed.
+
+  Lemma mem_store_cur:
+    forall chunk b ofs v m m',
+      Mem.store chunk m b ofs v = Some m' ->
+      forall b' ofs',
+        (getCurPerm m) # b' ofs' = (getCurPerm m') # b' ofs'.
+  Proof.
+    intros.
+    unfold Mem.store in *.
+    destruct (Mem.valid_access_dec m chunk b ofs Writable); try discriminate.
+    inversion H; subst.
+    do 2 rewrite getCurPerm_correct.
+    reflexivity.
+  Qed.
+
+  Lemma load_valid_block:
+    forall (m : mem) b ofs chunk v,
+      Mem.load chunk m b ofs = Some v ->
+      Mem.valid_block m b.
+  Proof.
+    intros m b ofs chunk v Hload.
+    apply Mem.load_valid_access in Hload.
+    apply Mem.valid_access_valid_block with (chunk:=chunk) (ofs:= ofs).
+    eapply Mem.valid_access_implies; eauto.
+    constructor.
+  Qed.
+  
+End MemoryLemmas.
